yalla/mll_ax_exp.v
@@ -1,0 +1,943 @@
+(* Expanding axioms in a proof net *)
+(* TODO remove unused imports *)
+From Coq Require Import Bool Wf_nat.
+From OLlibs Require Import dectype Permutation_Type_more.
+Set Warnings "-notation-overridden". (* to ignore warnings due to the import of ssreflect *)
+From mathcomp Require Import all_ssreflect zify.
+Set Warnings "notation-overridden".
+From GraphTheory Require Import preliminaries mgraph setoid_bigop structures bij.
+
+From Yalla Require Export graph_more mll_prelim mll_def mll_basic mll_seq_to_pn mll_correct.
+
+Import EqNotations.
+
+Set Mangle Names.
+Set Mangle Names Light.
+Set Implicit Arguments.
+Unset Strict Implicit.
+Unset Printing Implicit Defensive.
+Set Bullet Behavior "Strict Subproofs".
+
+
+
+Section Atoms.
+
+(** A set of atoms for building formulas *)
+Context { atom : DecType }.
+(* TODO meilleur moyen de récupérer les notations *)
+Notation formula := (@formula atom).
+Notation ll := (@ll atom).
+Notation base_graph := (graph (flat rule) (flat (formula * bool))).
+Notation graph_data := (@graph_data atom).
+Notation proof_structure := (@proof_structure atom).
+Notation proof_net := (@proof_net atom).
+
+
+(** ** The substitution in a proof net/structure of an atom by a proof net/structure
+       yields a proof net/structure *)
+
+(** Results on a proof structure with two conclusions *)
+Lemma subst_ax_conc_H_neq (H : proof_structure) (c1 c2 : edge H) (Ho : order H = [:: c1; c2]) :
+  c1 <> c2.
+Proof. destruct (p_order H) as [_ U]. revert U. rewrite Ho /= !in_cons. introb. Qed.
+
+Lemma subst_ax_conc_H_c (H : proof_structure) (c1 c2 : edge H) (Ho : order H = [:: c1; c2]) :
+  vlabel (target c1) = c /\ vlabel (target c2) = c.
+Proof. destruct (p_order H) as [O _]. split; apply O; rewrite /= Ho !in_cons; caseb. Qed.
+
+Lemma subst_ax_target_conc_H_neq (H : proof_structure) (c1 c2 : edge H) (Ho : order H = [:: c1; c2]) :
+  target c1 <> target c2.
+Proof.
+  intros ?.
+  enough (F : c1 = c2) by by apply subst_ax_conc_H_neq in F.
+  apply one_target_c; trivial.
+  apply (subst_ax_conc_H_c Ho).
+Qed.
+
+(* Graph where we replaced the axiom node v by the proof structure H *)
+(* Lemmas to simplify the definition by keeping their proofs opaque *)
+Lemma subst_ax_graph_0 (G : proof_structure) (v : G) (V : vlabel v = ax) (e : edge G) :
+  source e = source (ax_formula_edge V) -> target e \in [set~ v].
+Proof.
+  intro E.
+  rewrite !in_set -(ax_formula_edge_in V) -E.
+  apply /eqP. apply nesym, no_selfloop.
+Qed.
+
+Lemma subst_ax_graph_01 (G : proof_structure) (v : G) (V : vlabel v = ax) :
+  target (ax_formula_edge V) \in [set~ v].
+Proof. exact (subst_ax_graph_0 erefl). Qed.
+Lemma subst_ax_graph_02 (G : proof_structure) (v : G) (V : vlabel v = ax) :
+  target ((other_ax (ax_formula_endpoint V))) \in [set~ v].
+Proof. exact (subst_ax_graph_0 (other_ax_e (ax_formula_endpoint V))). Qed.
+
+Lemma subst_ax_graph_1 (H : proof_structure) (c1 c2 : edge H) (Ho : order H = [:: c1; c2]) :
+  source c1 \in setT :\ target c1 :\ target c2 /\
+  source c2 \in setT :\ target c1 :\ target c2.
+Proof.
+  rewrite !in_set. splitb; apply /eqP.
+  - apply no_source_c, (subst_ax_conc_H_c Ho).
+  - apply no_selfloop.
+  - apply no_selfloop.
+  - apply no_source_c, (subst_ax_conc_H_c Ho).
+Qed.
+
+Lemma subst_ax_graph_11 (H : proof_structure) (c1 c2 : edge H) (Ho : order H = [:: c1; c2]) :
+  source c1 \in setT :\ target c1 :\ target c2.
+Proof. by destruct (subst_ax_graph_1 Ho). Qed.
+Lemma subst_ax_graph_12 (H : proof_structure) (c1 c2 : edge H) (Ho : order H = [:: c1; c2]) :
+  source c2 \in setT :\ target c1 :\ target c2.
+Proof. by destruct (subst_ax_graph_1 Ho). Qed.
+
+Definition subst_ax_graph (G : proof_structure) (v : G) (V : vlabel v = ax)
+  (H : proof_structure) (c1 c2 : edge H) (Ho : order H = [:: c1; c2]) : base_graph :=
+  (remove_vertex v ⊎ induced (setT :\ target c1 :\ target c2))
+  ∔ [inr (Sub (source c1) (subst_ax_graph_11 Ho)), elabel (ax_formula_edge V),
+    inl (Sub (target (ax_formula_edge V)) (subst_ax_graph_01 V))]
+  ∔ [inr (Sub (source c2) (subst_ax_graph_12 Ho)), elabel (other_ax (ax_formula_endpoint V)),
+    inl (Sub (target (other_ax (ax_formula_endpoint V))) (subst_ax_graph_02 V))].
+
+Lemma subst_ax_G_removed (G : proof_structure) (v : G) (V : vlabel v = ax) :
+  edges_at v = [set ax_formula_edge V ; other_ax (ax_formula_endpoint V)].
+Proof.
+  apply /setP => e.
+  rewrite edges_at_eq -other_ax_set.
+  replace (target e == v) with false by by (symmetry; apply /eqP; apply no_target_ax).
+  by rewrite !in_set orb_false_r ax_cut_formula_edge_in.
+Qed.
+
+Lemma subst_ax_H_removed (H : proof_structure) (c1 c2 : edge H) (Ho : order H = [:: c1; c2]) :
+  edge_set (setT :\ target c1 :\ target c2) = setT :\ c1 :\ c2.
+Proof.
+  apply /setP => e.
+  rewrite !in_set !andb_true_r.
+  destruct (eq_comparable e c1) as [? | Neq1];
+  [ | destruct (eq_comparable e c2) as [? | Neq2]];
+  try (subst e; by rewrite !eq_refl /= !andb_false_r).
+  transitivity true; last by (symmetry; splitb; apply /eqP).
+  destruct (subst_ax_conc_H_c Ho).
+  splitb; apply /eqP.
+  - by apply no_source_c.
+  - by apply no_source_c.
+  - intros ?. contradict Neq2. by apply one_target_c.
+  - intros ?. contradict Neq1. by apply one_target_c.
+Qed.
+
+(* Inclusion of edges from G *)
+Definition subst_ax_incl_EG (G : proof_structure) (v : G) (V : vlabel v = ax)
+  (H : proof_structure) (c1 c2 : edge H) (Ho : order H = [:: c1; c2]) :
+  edge G -> edge (subst_ax_graph V Ho) :=
+  fun e => if @boolP (e \in ~: edges_at v) is AltTrue p then Some (Some (inl (Sub e p)))
+           else if e == ax_formula_edge V then Some None
+           else None.
+
+(* Last case in subst_ax_incl_EG *)
+Lemma subst_ax_incl_EG_other_edge (G : proof_structure) (v : G) (V : vlabel v = ax) (e : edge G) :
+  e \notin ~: edges_at v -> e <> ax_formula_edge V -> e = other_ax (ax_formula_endpoint V).
+Proof.
+  intros H ?.
+  apply other_ax_eq. split; trivial.
+  rewrite ax_formula_edge_in.
+  revert H. rewrite !in_set => /negPn/existsP[[] /eqP-H] //.
+  contradict H.
+  by apply no_target_ax.
+Qed.
+
+Lemma subst_ax_incl_EG_SS (G : proof_structure) (v : G) (V : vlabel v = ax)
+  (H : proof_structure) (c1 c2 : edge H) (Ho : order H = [:: c1; c2])
+  (e : edge G) (E : e \in ~: edges_at v) :
+  subst_ax_incl_EG V Ho e = Some (Some (inl (Sub e E))).
+Proof. unfold subst_ax_incl_EG. case: {-}_ /boolP => [? | /negP-? //]. cbnb. Qed.
+
+Lemma subst_ax_incl_EG_SN (G : proof_structure) (v : G) (V : vlabel v = ax)
+  (H : proof_structure) (c1 c2 : edge H) (Ho : order H = [:: c1; c2]) :
+  subst_ax_incl_EG V Ho (ax_formula_edge V) = Some None.
+Proof.
+  unfold subst_ax_incl_EG.
+  case: {-}_ /boolP => [In | ?]; [ | case_if].
+  contradict In. apply /negP.
+  rewrite subst_ax_G_removed !in_set.
+  apply /negPn. caseb.
+Qed.
+
+Lemma subst_ax_incl_EG_N (G : proof_structure) (v : G) (V : vlabel v = ax)
+  (H : proof_structure) (c1 c2 : edge H) (Ho : order H = [:: c1; c2]) :
+  subst_ax_incl_EG V Ho (other_ax (ax_formula_endpoint V)) = None.
+Proof.
+  unfold subst_ax_incl_EG.
+  case: {-}_ /boolP => [In | In].
+  - contradict In. apply /negP.
+    rewrite subst_ax_G_removed !in_set.
+    apply /negPn. caseb.
+  - case_if.
+    by assert (other_ax (ax_formula_endpoint V) <> ax_formula_edge V) by apply other_ax_neq.
+Qed.
+
+Lemma subst_ax_incl_EG_inj (G : proof_structure) (v : G) (V : vlabel v = ax)
+  (H : proof_structure) (c1 c2 : edge H) (Ho : order H = [:: c1; c2]) :
+  injective (subst_ax_incl_EG V Ho).
+Proof.
+  intros e f.
+  unfold subst_ax_incl_EG.
+  case: {-}_ /boolP => [E | E];
+  case: {-}_ /boolP => [F | F].
+  { intro Eq. by inversion Eq. }
+  all: case_if.
+  transitivity (other_ax (ax_formula_endpoint V)); [ | symmetry];
+  by apply subst_ax_incl_EG_other_edge.
+Qed.
+
+Lemma subst_ax_incl_EG_elabel (G : proof_structure) (v : G) (V : vlabel v = ax)
+  (H : proof_structure) (c1 c2 : edge H) (Ho : order H = [:: c1; c2]) (e : edge G) :
+  elabel (subst_ax_incl_EG V Ho e) = elabel e.
+Proof.
+  unfold subst_ax_incl_EG.
+  case: {-}_ /boolP => [// | In].
+  case_if.
+  f_equal.
+  symmetry. apply other_ax_eq. split; trivial.
+  rewrite ax_formula_edge_in.
+  revert In. rewrite !in_set => /negPn/existsP[[] /eqP-In] //.
+  contradict In.
+  by apply no_target_ax.
+Qed.
+
+Lemma subst_ax_incl_EG_flabel (G : proof_structure) (v : G) (V : vlabel v = ax)
+  (H : proof_structure) (c1 c2 : edge H) (Ho : order H = [:: c1; c2]) (e : edge G) :
+  flabel (subst_ax_incl_EG V Ho e) = flabel e.
+Proof. by rewrite /flabel subst_ax_incl_EG_elabel. Qed.
+
+Lemma subst_ax_incl_EG_llabel (G : proof_structure) (v : G) (V : vlabel v = ax)
+  (H : proof_structure) (c1 c2 : edge H) (Ho : order H = [:: c1; c2]) (e : edge G) :
+  llabel (subst_ax_incl_EG V Ho e) = llabel e.
+Proof. by rewrite /llabel subst_ax_incl_EG_elabel. Qed.
+
+Lemma subst_ax_incl_EG_edges_at (G : proof_structure) (v : G) (V : vlabel v = ax)
+  (H : proof_structure) (c1 c2 : edge H) (Ho : order H = [:: c1; c2])
+  (b : bool) (u : G) (U : u \in [set~ v]) :
+  edges_at_outin b (inl (Sub u U) : subst_ax_graph V Ho) =
+  [set subst_ax_incl_EG V Ho e | e in edges_at_outin b u].
+Proof.
+  apply setP => e.
+  rewrite in_set.
+  destruct (eq_comparable (endpoint b e) (inl (Sub u U))) as [Heq | Hneq]; symmetry.
+  - rewrite Heq eq_refl.
+    apply /imsetP.
+    destruct e as [[[[e E] | ?] | ] | ]; try by [].
+    + exists e.
+      * inversion Heq. apply endpoint_in_edges_at_outin.
+      * symmetry. apply subst_ax_incl_EG_SS.
+    + exists (ax_formula_edge V).
+      * destruct b; simpl in Heq; try by [].
+        inversion Heq. apply endpoint_in_edges_at_outin.
+      * symmetry. apply subst_ax_incl_EG_SN.
+    + exists (other_ax (ax_formula_endpoint V)).
+      * destruct b; simpl in Heq; try by [].
+        inversion Heq. apply endpoint_in_edges_at_outin.
+      * symmetry. apply subst_ax_incl_EG_N.
+  - transitivity false; last by (symmetry; by apply /eqP).
+    apply /imsetP.
+    intros [f F ?]. subst e.
+    revert F. rewrite in_set => /eqP-?. subst u.
+    revert Hneq.
+    unfold subst_ax_incl_EG.
+    case: {-}_ /boolP => [In | ]; [ | case_if].
+    + by move => /eqP; cbn; simpl => /eqP.
+    + destruct b.
+      * by replace U with (subst_ax_graph_01 V) in * by apply eq_irrelevance.
+      * clear - U. contradict U. apply /negP.
+        rewrite !in_set. apply /negPn/eqP.
+        apply ax_formula_edge_in.
+    + assert (f = other_ax (ax_formula_endpoint V)) by by apply subst_ax_incl_EG_other_edge.
+      subst f.
+      destruct b.
+      * by replace U with (subst_ax_graph_02 V) in * by apply eq_irrelevance.
+      * clear - U. contradict U. apply /negP.
+        rewrite !in_set other_ax_e. apply /negPn/eqP.
+        apply ax_formula_edge_in.
+Qed.
+
+(* Inclusion of edges from H *)
+Definition subst_ax_incl_EH (G : proof_structure) (v : G) (V : vlabel v = ax)
+  (H : proof_structure) (c1 c2 : edge H) (Ho : order H = [:: c1; c2]) :
+  edge H -> edge (subst_ax_graph V Ho) :=
+  fun e => if @boolP (e \in edge_set (setT :\ target c1 :\ target c2))
+    is AltTrue p then Some (Some (inr (Sub e p)))
+    else if e == c1 then Some None
+    else None.
+
+(* Last case in subst_ax_incl_EH *)
+Lemma subst_ax_incl_EH_other_edge (H : proof_structure) (c1 c2 : edge H) (Ho : order H = [:: c1; c2])
+  (e : edge H) :
+  e \notin edge_set (setT :\ target c1 :\ target c2) -> e <> c1 -> e = c2.
+Proof. rewrite subst_ax_H_removed // !in_set. introb. Qed.
+
+Lemma subst_ax_incl_EH_SS (G : proof_structure) (v : G) (V : vlabel v = ax)
+  (H : proof_structure) (c1 c2 : edge H) (Ho : order H = [:: c1; c2])
+  (e : edge H) (E : e \in edge_set (setT :\ target c1 :\ target c2)) :
+  subst_ax_incl_EH V Ho e = Some (Some (inr (Sub e E))).
+Proof. unfold subst_ax_incl_EH. case: {-}_ /boolP => [? | /negP-? //]. cbnb. Qed.
+
+Lemma subst_ax_incl_EH_SN (G : proof_structure) (v : G) (V : vlabel v = ax)
+  (H : proof_structure) (c1 c2 : edge H) (Ho : order H = [:: c1; c2]) :
+  subst_ax_incl_EH V Ho c1 = Some None.
+Proof.
+  unfold subst_ax_incl_EH.
+  case: {-}_ /boolP => [In | ?]; [ | case_if].
+  contradict In. apply /negP.
+  rewrite subst_ax_H_removed // !in_set. caseb.
+Qed.
+
+Lemma subst_ax_incl_EH_N (G : proof_structure) (v : G) (V : vlabel v = ax)
+  (H : proof_structure) (c1 c2 : edge H) (Ho : order H = [:: c1; c2]) :
+  subst_ax_incl_EH V Ho c2 = None.
+Proof.
+  unfold subst_ax_incl_EH.
+  case: {-}_ /boolP => [In | In].
+  - contradict In. apply /negP.
+    rewrite !in_set. caseb.
+  - case_if.
+    by assert (c1 <> c1) by apply (subst_ax_conc_H_neq Ho).
+Qed.
+
+Lemma subst_ax_incl_EH_inj (G : proof_structure) (v : G) (V : vlabel v = ax)
+  (H : proof_structure) (c1 c2 : edge H) (Ho : order H = [:: c1; c2]) :
+  injective (subst_ax_incl_EH V Ho).
+Proof.
+  intros e f.
+  unfold subst_ax_incl_EH.
+  case: {-}_ /boolP => [E | E];
+  case: {-}_ /boolP => [F | F].
+  { intro Eq. by inversion Eq. }
+  all: case_if.
+  transitivity c2; [ | symmetry];
+  by apply (subst_ax_incl_EH_other_edge Ho).
+Qed.
+
+Lemma subst_ax_incl_EH_edges_at (G : proof_structure) (v : G) (V : vlabel v = ax)
+  (H : proof_structure) (c1 c2 : edge H) (Ho : order H = [:: c1; c2])
+  (b : bool) (u : H) (U : u \in (setT :\ target c1 :\ target c2)) :
+  edges_at_outin b (inr (Sub u U) : subst_ax_graph V Ho) =
+  [set subst_ax_incl_EH V Ho e | e in edges_at_outin b u].
+Proof.
+  apply setP => e.
+  rewrite in_set.
+  destruct (eq_comparable (endpoint b e) (inr (Sub u U))) as [Heq | Hneq]; symmetry.
+  - rewrite Heq eq_refl.
+    apply /imsetP.
+    destruct e as [[[? | [e E]] | ] | ]; try by [].
+    + exists e.
+      * inversion Heq. apply endpoint_in_edges_at_outin.
+      * symmetry. apply subst_ax_incl_EH_SS.
+    + exists c1.
+      * destruct b; simpl in Heq; try by [].
+        inversion Heq. apply endpoint_in_edges_at_outin.
+      * symmetry. apply subst_ax_incl_EH_SN.
+    + exists c2.
+      * destruct b; simpl in Heq; try by [].
+        inversion Heq. apply endpoint_in_edges_at_outin.
+      * symmetry. apply subst_ax_incl_EH_N.
+  - transitivity false; last by (symmetry; by apply /eqP).
+    apply /imsetP.
+    intros [f F ?]. subst e.
+    revert F. rewrite in_set => /eqP-?. subst u.
+    revert Hneq.
+    unfold subst_ax_incl_EH.
+    case: {-}_ /boolP => [In | ]; [ | case_if].
+    + by move => /eqP; cbn; simpl => /eqP.
+    + destruct b.
+      * clear - U. contradict U. apply /negP.
+        rewrite !in_set. caseb.
+      * by replace U with (subst_ax_graph_11 Ho) in * by apply eq_irrelevance.
+    + assert (f = c2) by by apply (subst_ax_incl_EH_other_edge Ho).
+      subst f.
+      destruct b.
+      * clear - U. contradict U. apply /negP.
+        rewrite !in_set. caseb.
+      * by replace U with (subst_ax_graph_12 Ho) in * by apply eq_irrelevance.
+Qed.
+
+Lemma subst_ax_incl_EH_flabel (G : proof_structure) (v : G) (V : vlabel v = ax)
+  (H : proof_structure) (c1 c2 : edge H) (Ho : order H = [:: c1; c2]) (e : edge H) :
+  flabel c1 = flabel (ax_formula_edge V) ->
+  flabel c2 = (flabel (ax_formula_edge V))^ ->
+  flabel (subst_ax_incl_EH V Ho e) = flabel e.
+Proof.
+  intros F1 F2.
+  unfold subst_ax_incl_EH.
+  case: {-}_ /boolP => [// | In].
+  case_if.
+  assert (e = c2) as -> by by apply (subst_ax_incl_EH_other_edge Ho).
+  enough (F : flabel (other_ax (ax_formula_endpoint V)) = (flabel (ax_formula_edge V))^)
+    by by revert F; unfold flabel => ->.
+  apply other_ax_flabel.
+Qed.
+
+Lemma subst_ax_incl_EH_llabel (G : proof_structure) (v : G) (V : vlabel v = ax)
+  (H : proof_structure) (c1 c2 : edge H) (Ho : order H = [:: c1; c2]) (e : edge H) :
+  target e \in setT :\ target c1 :\ target c2 ->
+  llabel (subst_ax_incl_EH V Ho e) = llabel e.
+Proof.
+  intro E.
+  unfold subst_ax_incl_EH.
+  case: {-}_ /boolP => [// | In].
+  contradict In. apply /negP/negPn.
+  rewrite in_set E !in_set. splitb; apply /eqP.
+  all: apply no_source_c, (subst_ax_conc_H_c Ho).
+Qed.
+
+(* TODO Pour H et G : gros copié collé, comment factoriser ça ? fonction incl avec i : bool en param ? *)
+
+(** Graph data of an expanded axiom *)
+Definition subst_ax_graph_data (G : proof_structure) (v : G) (V : vlabel v = ax)
+  (H : proof_structure) (c1 c2 : edge H) (Ho : order H = [:: c1; c2]) : graph_data := {|
+  graph_of := _;
+  order := [seq subst_ax_incl_EG V Ho e | e <- order G];
+  |}.
+
+(** Proof structure of an expanded axiom *)
+Lemma subst_ax_p_deg (G : proof_structure) (v : G) (V : vlabel v = ax)
+  (H : proof_structure) (c1 c2 : edge H) (Ho : order H = [:: c1; c2]) :
+  proper_degree (subst_ax_graph V Ho).
+Proof.
+  unfold proper_degree.
+  intros b [[u U] | [u U]].
+  - rewrite -(p_deg b u) subst_ax_incl_EG_edges_at.
+    apply card_imset, subst_ax_incl_EG_inj.
+  - rewrite -(p_deg b u) subst_ax_incl_EH_edges_at.
+    apply card_imset, subst_ax_incl_EH_inj.
+Qed.
+
+Lemma subst_ax_p_ax_cut (G : proof_structure) (v : G) (V : vlabel v = ax)
+  (H : proof_structure) (c1 c2 : edge H) (Ho : order H = [:: c1; c2]) :
+  flabel c1 = flabel (ax_formula_edge V) ->
+  flabel c2 = (flabel (ax_formula_edge V))^ ->
+  proper_ax_cut (subst_ax_graph V Ho).
+Proof.
+  intros.
+  unfold proper_ax_cut.
+  move => b [[u U] | [u U]] /= Hl.
+  - destruct (p_ax_cut Hl) as [l [r [L [R LR]]]].
+    exists (subst_ax_incl_EG V Ho l), (subst_ax_incl_EG V Ho r).
+    rewrite !subst_ax_incl_EG_edges_at !subst_ax_incl_EG_flabel.
+    splitb; by apply imset_f.
+  - destruct (p_ax_cut Hl) as [l [r [L [R LR]]]].
+    exists (subst_ax_incl_EH V Ho l), (subst_ax_incl_EH V Ho r).
+    rewrite !subst_ax_incl_EH_edges_at !subst_ax_incl_EH_flabel //.
+    splitb; by apply imset_f.
+Qed.
+
+Lemma subst_ax_p_tens_parr (G : proof_structure) (v : G) (V : vlabel v = ax)
+  (H : proof_structure) (c1 c2 : edge H) (Ho : order H = [:: c1; c2]) :
+  flabel c1 = flabel (ax_formula_edge V) ->
+  flabel c2 = (flabel (ax_formula_edge V))^ ->
+  proper_tens_parr (subst_ax_graph V Ho).
+Proof.
+  intros F1 F2.
+  unfold proper_tens_parr.
+  move => b [[u U] | [u U]] /= Hl.
+  - destruct (p_tens_parr Hl) as [l [r [c [? [? [? [? [? ?]]]]]]]].
+    exists (subst_ax_incl_EG V Ho l), (subst_ax_incl_EG V Ho r), (subst_ax_incl_EG V Ho c).
+    rewrite !subst_ax_incl_EG_edges_at !subst_ax_incl_EG_flabel !subst_ax_incl_EG_llabel.
+    splitb; by apply imset_f.
+  - destruct (p_tens_parr Hl) as [l [r [c [L [? [R [? [? ?]]]]]]]].
+    exists (subst_ax_incl_EH V Ho l), (subst_ax_incl_EH V Ho r), (subst_ax_incl_EH V Ho c).
+    rewrite !subst_ax_incl_EH_edges_at !subst_ax_incl_EH_flabel //.
+    splitb; try by apply imset_f.
+    all: rewrite subst_ax_incl_EH_llabel //.
+    + by revert L; rewrite in_set => /eqP-->.
+    + by revert R; rewrite in_set => /eqP-->.
+Qed.
+
+Lemma subst_ax_p_noleft (G : proof_structure) (v : G) (V : vlabel v = ax)
+  (H : proof_structure) (c1 c2 : edge H) (Ho : order H = [:: c1; c2]) :
+  proper_noleft (subst_ax_graph V Ho).
+Proof.
+  intros [[[? | ?] | ] | ].
+  - apply p_noleft.
+  - apply p_noleft.
+  - rewrite /= -subst_ax_incl_EG_SN subst_ax_incl_EG_llabel.
+    apply p_noleft.
+  - rewrite /= -subst_ax_incl_EG_N subst_ax_incl_EG_llabel.
+    apply p_noleft.
+Qed.
+
+Lemma subst_ax_p_order (G : proof_structure) (v : G) (V : vlabel v = ax)
+  (H : proof_structure) (c1 c2 : edge H) (Ho : order H = [:: c1; c2]) :
+  proper_order (subst_ax_graph_data V Ho).
+Proof.
+  unfold proper_order. simpl order. split.
+  - intros [[[[e E] | [e E]] | ] | ]; simpl.
+    + rewrite -(subst_ax_incl_EG_SS V Ho) mem_map; last by apply subst_ax_incl_EG_inj.
+      apply p_order.
+    + assert (forall i, Some (Some (inr i)) \in [seq subst_ax_incl_EG V Ho u | u <- order G] = false)
+        as ->.
+      { intros ?.
+        apply /negP => /mapP[? _].
+        unfold subst_ax_incl_EG.
+        case: {-}_ /boolP; case_if. }
+      split => C //.
+      apply p_order in C.
+      contradict E. apply /negP.
+      revert C.
+      rewrite Ho /= !in_cons in_nil !in_set.
+      introb; caseb.
+    + rewrite -subst_ax_incl_EG_SN mem_map; last by apply subst_ax_incl_EG_inj.
+      apply p_order.
+    + rewrite -subst_ax_incl_EG_N mem_map; last by apply subst_ax_incl_EG_inj.
+      apply p_order.
+  - rewrite map_inj_uniq; last by apply subst_ax_incl_EG_inj.
+    apply p_order.
+Qed.
+
+Definition subst_ax_ps (G : proof_structure) (v : G) (V : vlabel v = ax)
+  (H : proof_structure) (c1 c2 : edge H) (Ho : order H = [:: c1; c2])
+  (F1 : flabel c1 = flabel (ax_formula_edge V))
+  (F2 : flabel c2 = (flabel (ax_formula_edge V))^) : proof_structure := {|
+  graph_data_of := subst_ax_graph_data V Ho;
+  p_deg := @subst_ax_p_deg _ _ _ _ _ _ _;
+  p_ax_cut := @subst_ax_p_ax_cut _ _ _ _ _ _ _ F1 F2;
+  p_tens_parr := @subst_ax_p_tens_parr _ _ _ _ _ _ _ F1 F2;
+  p_noleft := @subst_ax_p_noleft _ _ _ _ _ _ _;
+  p_order := subst_ax_p_order _ _;
+  |}.
+
+Fixpoint subst_ax_upath_bwd_G (G : proof_structure) (v : G) (V : vlabel v = ax)
+  (H : proof_structure) (c1 c2 : edge H) (Ho : order H = [:: c1; c2])
+  (p : @upath _ _ (subst_ax_graph V Ho)) : @upath _ _ G :=
+  match p with
+  | [::] => [::]
+  | (e, b) :: p' => match e with
+    | Some (Some (inl (exist e' _))) => [:: (e', b)]
+    | Some (Some (inr _)) => [::]
+    | Some None => [:: (ax_formula_edge V, b)]
+    | None => [:: (other_ax (ax_formula_endpoint V), b)]
+  end ++ subst_ax_upath_bwd_G p'
+end.
+
+(* méthode : si cycle c dans graph,
+alors expanse_ax_upath_bwd c cycle dans G;
+si expanse_ax_upath_bwd p vide, alors p inclut dans expanded_ax (ie p = Some Some inr p'
+et p' chem entre antécédents)
+donc si cycle c, alors cycle c' dans expanded, absurde *)
+
+Definition subst_ax_u_G (G : proof_structure) (v : G) (V : vlabel v = ax)
+  (H : proof_structure) (c1 c2 : edge H) (Ho : order H = [:: c1; c2])
+  (u : subst_ax_graph V Ho) : G :=
+  match u with
+  | inl (exist u _) => u
+  | _ => v
+  end.
+
+Lemma subst_ax_switching_eq (G : proof_structure) (v : G) (V : vlabel v = ax)
+  (H : proof_structure) (c1 c2 : edge H) (Ho : order H = [:: c1; c2])
+  (e f : edge G) :
+  switching e = switching f ->
+  switching (subst_ax_incl_EG V Ho e) = switching (subst_ax_incl_EG V Ho f).
+Proof.
+  move => /eqP.
+  unfold subst_ax_incl_EG.
+  case: {-}_ /boolP => [E | E];
+  case: {-}_ /boolP => [F | F];
+  unfold switching; case_if; cbnb; simpl in *.
+  all: try ((assert (f = other_ax (ax_formula_endpoint V)) by by apply subst_ax_incl_EG_other_edge);
+    subst f); try by [].
+  all: try ((assert (e = other_ax (ax_formula_endpoint V)) by by apply subst_ax_incl_EG_other_edge);
+    subst e); try by [].
+  all: try by assert (~ eqb_rule (vlabel (target (ax_formula_edge V))) (⅋)) by by apply /negP.
+  all: try by assert (~ eqb_rule (vlabel (target (other_ax (ax_formula_endpoint V)))) (⅋)) by by apply /negP.
+  all: try by contradict E; apply /negP.
+  all: try by contradict F; apply /negP.
+Qed.
+(* TODO 100 cas, long *)
+
+Lemma subst_ax_image_in (G : proof_structure) (v : G) (V : vlabel v = ax)
+  (H : proof_structure) (c1 c2 : edge H) (Ho : order H = [:: c1; c2])
+  (p : upath) (e : edge G) (b : bool) :
+  (e, b) \in subst_ax_upath_bwd_G p -> (subst_ax_incl_EG V Ho e, b) \in p.
+Proof.
+  revert e b. induction p as [ | (f, fb) p IH] => e eb //=.
+  rewrite in_cons mem_cat.
+  move => /orP[In | ?]; apply /orP; [left | right; by apply IH].
+  destruct f as [[[[f F] | f] | ] | ].
+  all: revert In; rewrite ?in_cons in_nil ?orb_false_r => /eqP-In //.
+  all: inversion In; clear In; subst e eb.
+  - by rewrite subst_ax_incl_EG_SS.
+  - by rewrite subst_ax_incl_EG_SN.
+  - by rewrite subst_ax_incl_EG_N.
+Qed.
+
+Lemma subst_ax_switching_notin (G : proof_structure) (v : G) (V : vlabel v = ax)
+  (H : proof_structure) (c1 c2 : edge H) (Ho : order H = [:: c1; c2])
+  (p : upath) (e : edge G) :
+  switching (subst_ax_incl_EG V Ho e) \notin [seq switching f.1 | f <- p] ->
+  switching e \notin [seq switching f.1 | f <- subst_ax_upath_bwd_G p].
+Proof.
+  intro Nin.
+  apply /mapP.
+  intros [(f, b) F EF].
+  contradict Nin. apply /negP/negPn/mapP.
+  exists (subst_ax_incl_EG V Ho f, b).
+  - by apply subst_ax_image_in.
+  - by apply subst_ax_switching_eq.
+Qed.
+
+Lemma subst_ax_switching_eq_SSR (G : proof_structure) (v : G) (V : vlabel v = ax)
+  (H : proof_structure) (c1 c2 : edge H) (Ho : order H = [:: c1; c2])
+  (e f : edge H)
+  (E : e \in edge_set (setT :\ target c1 :\ target c2))
+  (F : f \in edge_set (setT :\ target c1 :\ target c2)) :
+  switching e = switching f ->
+  switching (Some (Some (inr (Sub e E))) : edge (subst_ax_graph V Ho)) =
+    switching (Some (Some (inr (Sub f F))) : edge (subst_ax_graph V Ho)).
+Proof. move => /eqP. unfold switching; case_if; cbnb. Qed.
+
+Lemma subst_ax_supath_bwd (G : proof_structure) (v : G) (V : vlabel v = ax)
+  (H : proof_structure) (c1 c2 : edge H) (Ho : order H = [:: c1; c2])
+  (p : upath) (s t : subst_ax_graph V Ho) :
+  supath switching s t p ->
+  supath switching (subst_ax_u_G s) (subst_ax_u_G t) (subst_ax_upath_bwd_G p).
+Proof.
+  revert s t. induction p as [ | (e, b) p IH] => s t.
+  { move => /andP[/andP[/eqP-? _] _]. subst. apply supath_nilK. }
+  rewrite /supath /= !in_cons !map_cat cat_uniq mem_cat !negb_orb.
+  move => /andP[/andP[/andP[/eqP-? W] /andP[u U]] /andP[/eqP-n N]]. subst s.
+  assert (P : supath switching (endpoint b e) t p) by splitb.
+  revert IH => /(_ _ _ P) {W U N P} /andP[/andP[W2 ->] ->]. splitb.
+  - eapply (uwalk_cat _ W2). Unshelve.
+    destruct e as [[[[e E] | e] | ] | ], b; simpl; splitb;
+    by rewrite ?other_ax_e ax_formula_edge_in.
+  - by destruct e as [[[[e E] | e] | ] | ].
+  - destruct e as [[[[e E] | e] | ] | ];
+    rewrite has_sym //= orb_false_r;
+    apply subst_ax_switching_notin.
+    + by rewrite subst_ax_incl_EG_SS.
+    + by rewrite subst_ax_incl_EG_SN.
+    + by rewrite subst_ax_incl_EG_N.
+  - by destruct e as [[[[? ?] | ?] | ] | ].
+Qed.
+
+Lemma subst_ax_upath_bwd_empty (G : proof_structure) (v : G) (V : vlabel v = ax)
+  (H : proof_structure) (c1 c2 : edge H) (Ho : order H = [:: c1; c2])
+  (p : @upath _ _ (subst_ax_graph V Ho)) :
+  subst_ax_upath_bwd_G p = [::] ->
+  {p' | p = [seq (Some (Some (inr e.1)), e.2) | e <- p']}.
+Proof.
+  induction p as [ | (e, b) p IH].
+  { intros _. by exists [::]. }
+  move => /= /eqP. rewrite cat_nil => /andP[/eqP-E /eqP-P].
+  destruct (IH P) as [p' ?]. subst p. clear IH P.
+  destruct e as [[[[? ?] | e] | ] | ]; try by []. clear E.
+  by exists ((e, b) :: p').
+Qed.
+
+Definition subst_ax_upath_bwd_empty' (G : proof_structure) (v : G) (V : vlabel v = ax)
+  (H : proof_structure) (c1 c2 : edge H) (Ho : order H = [:: c1; c2])
+  (p : @upath _ _ (subst_ax_graph V Ho)) (P : subst_ax_upath_bwd_G p = [::]) : upath :=
+  [seq (val e.1,e.2) | e <- projT1 (subst_ax_upath_bwd_empty P)].
+
+Lemma subst_ax_supath_bwd_empty (G : proof_structure) (v : G) (V : vlabel v = ax)
+  (H : proof_structure) (c1 c2 : edge H) (Ho : order H = [:: c1; c2])
+  (p : upath) (P : subst_ax_upath_bwd_G p = [::]) (s t : subst_ax_graph V Ho) :
+  supath switching s t p -> p <> [::] ->
+  { '(s', t') | s = inr s' /\ t = inr t' /\ supath switching (val s') (val t') (subst_ax_upath_bwd_empty' P)}.
+Proof.
+  unfold subst_ax_upath_bwd_empty'.
+  destruct (subst_ax_upath_bwd_empty P) as [p' ?]. clear P. subst p. simpl.
+  destruct s as [s | s].
+  { by destruct p'. }
+  destruct t as [t | t].
+  { move => /andP[/andP[W _] _]. contradict W.
+    case/lastP: p' => [// | ? ?]. by rewrite map_rcons uwalk_rcons => /andP[_ ?]. }
+  intros P' _.
+  exists (s, t). split; [ | split]; trivial.
+  revert s t P'. induction p' as [ | ([e E], b) p' IH] => // [[s S] t].
+  rewrite /supath /= in_cons SubK'. cbn. rewrite SubK => /andP[/andP[/andP[/eqP-? ?] /andP[u' ?]] ?].
+  subst s.
+  assert (P' : supath switching (inr (Sub (endpoint b e) (induced_proof b E)) : subst_ax_graph V Ho)
+    (inr t) [seq (Some (Some (inr e.1)), e.2) | e <- p']) by splitb.
+  revert IH => /(_ _ _ P') {P'} /andP[/andP[-> ->] ->].
+  clear - u'. splitb.
+  rewrite -map_comp {b}.
+  apply /negP. move => /mapP[f Fin EF].
+  contradict u'. apply /negP/negPn.
+  rewrite -map_comp. apply /mapP.
+  exists f; trivial.
+  revert EF. simpl.
+  destruct f as ([f F], bf).
+  apply subst_ax_switching_eq_SSR.
+Qed.
+
+Lemma subst_ax_uacyclic (G : proof_structure) (v : G) (V : vlabel v = ax)
+  (H : proof_structure) (c1 c2 : edge H) (Ho : order H = [:: c1; c2]) :
+  uacyclic (@switching _ G) -> uacyclic (@switching _ H) ->
+  uacyclic (@switching _ (subst_ax_graph V Ho)).
+Proof.
+  move => AG AH u [p P]. cbnb. apply /eqP/negPn/negP => /eqP-?.
+  revert AG => /(_ _ {| upval := _ ; upvalK := subst_ax_supath_bwd P |}) /eqP. cbn =>/eqP-AG.
+  destruct (subst_ax_supath_bwd_empty AG P) as [[s' t'] [S [T P']]]; first by by [].
+  subst u. inversion T. clear T. subst t'.
+  unfold subst_ax_upath_bwd_empty' in P'.
+  destruct (subst_ax_upath_bwd_empty AG) as [p' ?]. subst p. simpl in P'.
+  revert AH => /(_ _ {| upval := _ ; upvalK := P' |}) /eqP. cbn => /eqP/eqP.
+  rewrite map_nil => /eqP-?. by subst p'.
+Qed.
+
+Lemma subst_ax_nb_vertices (G : proof_structure) (v : G) (V : vlabel v = ax)
+  (H : proof_structure) (c1 c2 : edge H) (Ho : order H = [:: c1; c2]) :
+  #|G| + #|H| = #|subst_ax_graph V Ho| + 3.
+Proof.
+  rewrite /subst_ax_graph /= card_sum card_set_subset card_set_subset !setE cardsC1.
+  rewrite -(cardsE H) (cardsD1 (target c1)) (cardsD1 (target c2)) cardsE.
+  rewrite !in_set /=.
+  replace (target c2 != target c1) with true
+    by (symmetry; apply /eqP; apply nesym, (subst_ax_target_conc_H_neq Ho)).
+  assert (#|G| <> 0) by by apply fintype0.
+  simpl in *. lia.
+Qed.
+
+Lemma subst_ax_nb_edges (G : proof_structure) (v : G) (V : vlabel v = ax)
+  (H : proof_structure) (c1 c2 : edge H) (Ho : order H = [:: c1; c2]) :
+  #|edge G| + #|edge H| = #|edge (subst_ax_graph V Ho)| + 2.
+Proof.
+  rewrite /= !card_option card_sum /= subst_ax_G_removed subst_ax_H_removed // !card_set_subset
+    !setE setC2.
+  rewrite -cardsT (cardsD1 (ax_formula_edge V)) (cardsD1 (other_ax (ax_formula_endpoint V))).
+  rewrite -cardsT (cardsD1 c1) (cardsD1 c2).
+  rewrite !in_set /=.
+  replace (other_ax (ax_formula_endpoint V) != ax_formula_edge V) with true
+    by by (symmetry; apply /eqP; apply other_ax_neq).
+  replace (c2 != c1) with true
+    by by (symmetry; apply /eqP; apply nesym, subst_ax_conc_H_neq).
+  lia.
+Qed.
+
+Lemma subst_ax_nb_parr (G : proof_structure) (v : G) (V : vlabel v = ax)
+  (H : proof_structure) (c1 c2 : edge H) (Ho : order H = [:: c1; c2]) :
+  #|[set u : G | vlabel u == ⅋]| + #|[set u : H | vlabel u == ⅋]| = #|[set u : subst_ax_graph V Ho | vlabel u == ⅋]|.
+Proof.
+  rewrite cards_sum_pred. f_equal.
+  - by rewrite (cards_subgraph_pred _ (fun x => vlabel x == ⅋)) set1CI (cardsD1 v) in_set V.
+  - rewrite (cards_subgraph_pred (@induced_proof _ _ _ _) (fun x => vlabel x == ⅋)) !setIDA setIT.
+    rewrite (cardsD1 (target c1)) (cardsD1 (target c2)) !in_set.
+    destruct (subst_ax_conc_H_c Ho) as [-> ->].
+    replace (target c2 != target c1) with true
+      by (symmetry; apply /eqP; apply nesym, (subst_ax_target_conc_H_neq Ho)).
+    simpl. lia.
+Qed.
+
+Lemma subst_ax_uconnected_nb (G : proof_structure) (v : G) (V : vlabel v = ax)
+  (H : proof_structure) (c1 c2 : edge H) (Ho : order H = [:: c1; c2]) :
+  flabel c1 = flabel (ax_formula_edge V) ->
+  flabel c2 = (flabel (ax_formula_edge V))^ ->
+  uacyclic (@switching _ G) -> uacyclic (@switching _ H) ->
+  uconnected_nb (@switching_left _ (subst_ax_graph V Ho)) + 1 =
+  uconnected_nb (@switching_left _ G) + uconnected_nb (@switching_left _ H).
+Proof.
+  move => F1 F2 AG AH.
+  assert (NG := switching_left_uconnected_nb AG).
+  assert (NH := switching_left_uconnected_nb AH).
+  assert (N := @switching_left_uconnected_nb atom (subst_ax_ps Ho F1 F2) (subst_ax_uacyclic AG AH)).
+  assert (X0 := subst_ax_nb_vertices V Ho).
+  assert (X1 := subst_ax_nb_edges V Ho).
+  assert (X2 := subst_ax_nb_parr V Ho).
+  simpl in *. lia.
+Qed.
+
+Lemma subst_ax_correct (G : proof_structure) (v : G) (V : vlabel v = ax)
+  (H : proof_structure) (c1 c2 : edge H) (Ho : order H = [:: c1; c2]) :
+  flabel c1 = flabel (ax_formula_edge V) ->
+  flabel c2 = (flabel (ax_formula_edge V))^ ->
+  correct G -> correct H -> correct (subst_ax_graph V Ho).
+Proof.
+  intros F1 F2 [AG CG] [AH CH]. split.
+  - by apply subst_ax_uacyclic.
+  - assert (N := subst_ax_uconnected_nb Ho F1 F2 AG AH). lia.
+Qed.
+
+Definition subst_ax_pn (G : proof_net)(v : G) (V : vlabel v = ax)
+  (H : proof_net) (c1 c2 : edge H) (Ho : order H = [:: c1; c2])
+  (F1 : flabel c1 = flabel (ax_formula_edge V))
+  (F2 : flabel c2 = (flabel (ax_formula_edge V))^) : proof_net := {|
+  ps_of := subst_ax_ps Ho F1 F2;
+  p_correct := subst_ax_correct Ho F1 F2 (p_correct G) (p_correct H);
+  |}.
+
+(** Sequent of an expanded axiom *)
+Lemma subst_ax_sequent (G : proof_structure) (v : G) (V : vlabel v = ax)
+  (H : proof_structure) (c1 c2 : edge H) (Ho : order H = [:: c1; c2]) :
+  sequent (subst_ax_graph_data V Ho) = sequent G.
+Proof.
+  rewrite /sequent -map_comp.
+  apply eq_map => e.
+  by rewrite /= subst_ax_incl_EG_flabel.
+Qed.
+
+Lemma subst_ax_proofs (H : graph_data) (A B : formula) :
+  sequent H = [:: A ; B] ->
+  {'(c1, c2) | order H = [:: c1; c2] /\ flabel c1 = A /\ flabel c2 = B}.
+Proof.
+  unfold sequent.
+  destruct (order H) as [ | c1 [ | c2 [ | ? ?]]];
+  cbn; rewrite ?andb_false_r //.
+  intro Ho. inversion Ho.
+  by exists (c1, c2).
+Qed.
+
+Definition subst_ax_ps_seq (G : proof_structure) (v : G) (V : vlabel v = ax)
+  (H : proof_structure) (Hs : sequent H = [:: flabel (ax_formula_edge V) ; (flabel (ax_formula_edge V))^]) :
+  proof_structure.
+Proof. destruct (subst_ax_proofs Hs) as [(c1, c2) [Ho [F1 F2]]]. exact (subst_ax_ps Ho F1 F2). Defined.
+
+
+(** ** Graph of an expanded axiom - all steps at once *)
+Lemma ax_expanded_all_0 (G : proof_structure) (v : G) (V : vlabel v = ax) (A B : formula) :
+  ax_formula V = A ⊗ B ->
+  sequent (pn (ax_exp (B^ ⅋ A^))) = [:: flabel (ax_formula_edge V) ; (flabel (ax_formula_edge V))^].
+Proof. by rewrite ps_consistent /= !bidual /ax_formula => ->. Qed.
+
+Definition ax_expanded_all (G : proof_structure) (v : G) (V : vlabel v = ax) (A B : formula) (F : ax_formula V = A ⊗ B) :
+  proof_structure := subst_ax_ps_seq (ax_expanded_all_0 F).
+
+(** ** Graph of an expanded axiom - one step *)
+Definition Permutation_Type_2_def {A : Type} (a b : A) : Permutation_Type [:: a; b] [:: b; a] :=
+  Permutation_Type_swap b a [::].
+
+Definition Permutation_Type_3_def {A : Type} (a b c : A) : Permutation_Type [:: a; b; c] [:: b; c; a].
+Proof.
+  etransitivity. apply Permutation_Type_swap.
+  apply Permutation_Type_skip, Permutation_Type_swap.
+Defined.
+
+Lemma expanded_ax_step0 (A B : formula) :
+  exists e0 l0 e1 l1,
+  order (ax_pn (A^)) = e0 :: l0 /\ order (ax_pn (B^)) = e1 :: l1.
+Proof. simpl. by exists ord0, [:: ord1], ord0, [:: ord1]. Qed.
+
+(** * Graph of two axioms A B linked by a tensor A ⊗ B *)
+Definition ax_expanded_tens (A B : formula) : proof_net :=
+  add_node_pn_tens (expanded_ax_step0 A B).
+Lemma ax_expanded_tens_sequent (A B : formula) :
+  sequent (ax_expanded_tens A B) = [:: A ⊗ B; B^; A^].
+Proof. rewrite (@add_node_sequent atom). cbn. by rewrite !bidual. Qed.
+
+Definition ax_expanded_tens_perm (A B : formula) :=
+  perm_pn (ax_expanded_tens A B) (Permutation_Type_3_def (A ⊗ B) (B^) (A^)).
+Lemma ax_expanded_tens_perm_sequent (A B : formula) :
+  sequent (ax_expanded_tens_perm A B) = [:: B^; A^; A ⊗ B].
+Proof. apply perm_sequent, ax_expanded_tens_sequent. Qed.
+
+Lemma expanded_ax_step1' (A B : formula) :
+  { '(e0, e1, e2) | order (ax_expanded_tens_perm A B) = [:: e0; e1; e2]
+  /\ val e0 = Some (Some (inl (inr ord1))) /\ val e1 = Some (Some (inl (inl ord1)))
+  /\ val e2 = Some (Some (inr None))}.
+Proof.
+  rewrite /= /add_node_order.
+  destruct (all_sigP _) as [l L].
+  assert (Hr : sval (exist (fun _ => _) l L) = l) by cbnb. (* TODO ce lemme doit exister *)
+  rewrite Hr {Hr}.
+  revert L. rewrite /add_node_order_2 /add_node_type_order /add_node_order_1 /=.
+  destruct l as [ | [l0 L0] [ | [l1 L1] [ | [l2 L2] [ | ? ?]]]]; try by []; simpl.
+  intro L. inversion L. subst.
+  by exists ((Sub _ L1), (Sub _ L2), (Sub _ L0)).
+Qed.
+
+Lemma expanded_ax_step1 (A B : formula) :
+  exists e0 e1 l, order (ax_expanded_tens_perm A B) = [:: e0, e1 & l].
+Proof.
+  destruct (expanded_ax_step1' A B) as [[[e0 e1] e2] [? _]].
+  by exists e0, e1, [:: e2].
+Qed.
+
+Definition ax_expanded (A B : formula) := perm_pn (add_node_pn_parr (expanded_ax_step1 A B))
+  (Permutation_Type_2_def (B^ ⅋ A^) (A ⊗ B)).
+Lemma ax_expanded_sequent (A B : formula) :
+  sequent (ax_expanded A B) = [:: A ⊗ B; B^ ⅋ A^].
+Proof.
+  rewrite perm_sequent // add_node_sequent.
+  destruct (expanded_ax_step1' A B) as [[[[? ?] [? ?]] [? ?]] [O [? [? ?]]]].
+  rewrite !O {O} ax_expanded_tens_perm_sequent. simpl in *. by subst.
+Qed.
+
+Lemma ax_expanded_one_0 (G : proof_structure) (v : G) (V : vlabel v = ax) (A B : formula) :
+  ax_formula V = A ⊗ B ->
+  sequent (ax_expanded A B) = [:: flabel (ax_formula_edge V) ; (flabel (ax_formula_edge V))^].
+Proof. by rewrite ax_expanded_sequent /ax_formula => ->. Qed.
+
+
+Definition ax_expanded_one (G : proof_structure) (v : G) (V : vlabel v = ax) (A B : formula) (F : ax_formula V = A ⊗ B) :
+  proof_structure := subst_ax_ps_seq (ax_expanded_one_0 F).
+
+(* TODO définir transformation rendant un réseau ax_atomic : par induction
+sur ax_formula *)
+
+(** Rewriting to expanse axioms *)
+Definition is_atomicb (A : formula) :=
+  if A is var _ then true else false.
+
+Definition is_ax_atomic (G : proof_structure) (v : G) :=
+  if @boolP (vlabel v == ax) is AltTrue V then is_atomicb (ax_formula (eqP V))
+  else true.
+
+Lemma expanse_term (G : proof_structure) :
+  {ax_atomic G} + {exists v : G, ~~ is_ax_atomic v}.
+Proof.
+  destruct [exists v : G, ~~ is_ax_atomic v] eqn:H.
+  { right. apply /existsP. exact H. }
+  left.
+  intros v V.
+  revert H => /existsPn/(_ v)/negPn.
+  unfold is_ax_atomic.
+  case: {-}_ /boolP => [H | H].
+  2:{ contradict H. by apply /negP/negPn/eqP. }
+  replace (eqP H) with V by apply eq_irrelevance. clear H.
+  unfold is_atomic, is_atomicb.
+  by destruct (ax_formula V) eqn:F.
+Qed.
+
+(* TODO define the quantity which decrease: sum of the size of formulas on axioms ? *)
+(* Show it decrease when expanding *)(*
+Lemma expanse_one_nb (G : proof_structure) (v : G) (V : vlabel v = ax) (A B : formula)
+  (VAB : flabel (ax_formula_edge V) = A ⊗ B) :
+  #|expanse_ax_ps VAB| < #|G|.
+Proof. (* TODO with good measure *)
+Admitted.*)
+
+(** All steps *)(*
+Lemma expanse_all (G : proof_structure) :
+  {P : proof_structure | correct G -> correct P & sequent P = sequent G /\ ax_atomic P}.
+(* TODO these properties are sufficient? *)
+Proof.
+  revert G.
+  enough (Hm : forall n (G : proof_structure), #|G| = n ->
+    {P : proof_structure | correct G -> correct P & sequent P = sequent G /\ ax_atomic P})
+    by (intro G; by apply (Hm #|G|)).
+  intro n; induction n as [n IH] using lt_wf_rect; intros G Hc.
+  have [/has_cutP/existsP/sigW[v /eqP-Hcut] | /has_cutP-?] := altP (has_cutP G).
+  2:{ by exists G. }
+  assert (N : (#|red_one_ps Hcut| < n)%coq_nat) by (rewrite -Hc; apply /leP; apply red_one_nb).
+  specialize (IH _ N _ erefl). destruct IH as [P CC [S C]].
+  exists P; [ | split; trivial].
+  - move => ?. by apply CC, red_one_correct.
+  - rewrite S. apply red_one_sequent.
+Qed.
+
+Definition red (G : proof_structure) : proof_structure := proj1_sig (red_all G).
+
+Lemma red_correct (G : proof_structure) : correct G -> correct (red G).
+Proof. by destruct (proj2_sig (red_all G)) as [? _]. Qed.
+
+Definition red_pn (G : proof_net) : proof_net := {|
+  ps_of := red G;
+  p_correct := red_correct (p_correct G);
+  |}.
+
+Lemma red_sequent (G : proof_structure) : sequent (red G) = sequent G.
+Proof. by destruct (proj2_sig (red_all G)) as [_ [? _]]. Qed.
+
+Lemma red_has_cut (G : proof_structure) : ~ has_cut (red G).
+Proof. by destruct (proj2_sig (red_all G)) as [_ [_ ?]]. Qed.
+
+(* TODO et definir une etape, puis repetition, idem cut *)
+*)
+End Atoms.
